# **Day 10: Equivalence of Functional Dependencies (FDs) in DBMS**

---

## **1. Introduction**

Two sets of functional dependencies (FDs) are **equivalent** if they enforce the **same constraints** on a relation.

Formally:

* Every FD in one set can be **derived** from the other set using **inference rules** (like Armstrong's axioms) and vice versa.
* Equivalent FDs preserve the **same data integrity**.

---

## **2. Why Check Equivalence of FDs?**

* Different designers may produce different FD sets for the same relation.
* Ensures the database design uses a **consistent and optimal set** of FDs.
* Helps in **normalization**, **removing redundancies**, and **optimizing database performance**.

---

## **3. How to Determine Equivalence**

Let **FD1** and **FD2** be two FD sets for relation `R`.

![](https://media.geeksforgeeks.org/wp-content/uploads/20230622164350/ezgifcom-gif-maker-(10).webp)

1. If all FDs of **FD1** can be derived from **FD2**, then:

   * `FD2 ⊃ FD1`

2. If all FDs of **FD2** can be derived from **FD1**, then:

   * `FD1 ⊃ FD2`

3. If both conditions hold, then:

   * `FD1 = FD2` → sets are **equivalent**

**Venn diagram representation:**

* Shows overlap and containment of FDs between two sets.

---

## **4. Advantages**

* Identify **redundant FDs** that can be removed
* Optimize database design with **interchangeable FD sets**
* Ensure **data consistency** across all derived attribute combinations

---

## **5. Disadvantages**

* Can be **computationally expensive**, especially for large datasets
* Requires testing **multiple candidate FD sets**, which is **time-consuming**
* May not reflect the **true semantic meaning** of data relationships

---

## **6. Examples**

### **Example 1: Equivalent FD Sets**

* Relation: `R(A,B,C,D)`
* FD1 = `{A → B, B → C, AB → D}`
* FD2 = `{A → B, B → C, A → C, A → D}`

**Step 1:** Check if all FDs of FD1 hold in FD2

* `A → B` ✅
* `B → C` ✅
* `AB → D` → `(AB)+ = {A,B,C,D}` in FD2 → ✅

**Step 2:** Check if all FDs of FD2 hold in FD1

* `A → B` ✅
* `B → C` ✅
* `A → C` → `(A)+ = {A,B,C,D}` in FD1 → ✅
* `A → D` → `(A)+ = {A,B,C,D}` in FD1 → ✅

**Conclusion:**

* `FD2 ⊃ FD1` and `FD1 ⊃ FD2` → **FD1 = FD2** → **Equivalent**

---

### **Example 2: Non-Equivalent FD Sets**

* Relation: `R2(A,B,C,D)`
* FD1 = `{A → B, B → C, A → C}`
* FD2 = `{A → B, B → C, A → D}`

**Step 1:** Check if all FDs of FD1 hold in FD2

* `A → B` ✅
* `B → C` ✅
* `A → C` → `(A)+ = {A,B,C,D}` in FD2 → ✅ → `FD2 ⊃ FD1`

**Step 2:** Check if all FDs of FD2 hold in FD1

* `A → B` ✅
* `B → C` ✅
* `A → D` → `(A)+ = {A,B,C}` in FD1 → ❌

**Conclusion:**

* `FD2 ⊃ FD1` but `FD2 ⊄ FD1` → **Not equivalent**
